#+PROPERTY: header-args:R :results none

* ProbTheory.jl
A script aiming to visualize basic probability theory concepts.

#+begin_src sh :results none :async
julia -e "include(\"ProbTheory.jl\");
          LLN();
          CLT();
          BE_binom_heatmap();
          BE_binom_slice()"
#+end_src

#+begin_comment
currently ess isn't working with org-babel

#+LATEX_CLASS: notes
#+LATEX_HEADER: \usepackage{fontspec}
#+LATEX_HEADER: \setmainfont[]{IBM Plex Sans}
#+LATEX_HEADER: \setmonofont[]{Iosevka SS14}
#+end_comment
* Law of Large Numbers

#+CAPTION: LLN (n = 600)
[[file:./media/LLN.gif]]
* Central Limit Theorem - Classical

#+CAPTION: CLT (n = 600)
[[file:./media/CLT.gif]]
* Berry-Esseen Theorem - Binomial Case

#+CAPTION: Binomial BE Heatmap (n = 500, tightbound)
[[file:./media/BE_binom_heatmap_500.png]]

#+CAPTION: Binomial BE Slice (n = 20, tightbound)
[[file:./media/BE_binom_slice.png]]

NOTE
When writing about BE,
Need to show what ksdistance is
by plotting the two cdfs and line between
for n = 5, 10, 50, ...


#+begin_src sh :results output
julia -e "include(\"ProbTheory.jl\"); BE_binom_bounds(1000)"
#+end_src

#+RESULTS:
: For n = 1000 on p = [0.001, 0.999], there are 183 negative differences.
: For n = 1000 on p = [0.333, 0.666], there are 0 negative differences.


* Appendix
** Reference
$$$E[X] = \int_{-\infty}^\infty xf(x)dx$$

$$f(x) = \frac{1}{b-a}$$

** Expectations
$$E[X] = \int_a^b x \frac{1}{b-a} = \frac{1}{2(b-a)} [x^2]_a^b = \frac{a+b}{2}$$

$$E[X^2] = \int_a^b x^2 \frac{1}{b-a} = \frac{1}{3(b-a)} [x^3]_a^b = \frac{(b-a)(b^2 + ba + a^2)}{3(b-a)} = \frac{b^2 + ba + a^2}{3}$$

** Checking the Variance

$$Var(X) = E[X^2] - E[X]^2$$

$$Var(X) = \frac{b^2 + ba + a^2}{3} - (\frac{a+b}{2})^2$$

$$Var(X) = \frac{b^2 + ba + a^2}{3} - \frac{a^2+2ab+b^2}{4}$$

$$Var(X) = \frac{4b^2 + 4ba + 4a^2}{12} - \frac{3a^2+6ab+3b^2}{12}$$

$$Var(X) = \frac{b^2 - 2ba + a^2}{12} = \frac{(b-a)^2}{12}$$

** E[|X|^3]

$$E[|X|^3] = \int_a^b |x|^3 \frac{1}{b-a}$$

$$ = \frac{1}{b-a} (\int_a^0 -x^3  + \int_0^b x^3)$$

$$ = \frac{1}{b-a} (-\frac{1}{4}[x^4]_a^0  + \frac{1}{4}[x^4]_0^b)$$

$$ = \frac{1}{b-a} (\frac{1}{4}a^4  + \frac{1}{4}b^4)$$

$$ = \frac{1}{4} \frac{1}{b-a} (a^4  + b^4)$$
